Foundation/InterpretabilityLogic/Veltman/Logic/ILMinus_J5.lean
@@ -1,0 +1,65 @@
+import Foundation.InterpretabilityLogic.Veltman.Logic.ILMinus
+import Foundation.InterpretabilityLogic.Veltman.AxiomJ5
+
+
+namespace LO.InterpretabilityLogic
+
+open Veltman
+
+
+namespace Veltman
+
+protected abbrev FrameClass.ILMinus_J5 : FrameClass := { F | F.HasAxiomJ5 }
+
+instance : trivialFrame.HasAxiomJ5 where
+  S_J5 _ := by tauto
+
+end Veltman
+
+
+open Hilbert.Minimal
+
+namespace ILMinus_J5
+
+instance Veltman.sound : Sound InterpretabilityLogic.ILMinus_J5 FrameClass.ILMinus_J5 := by
+  apply Veltman.instFrameClassSound;
+  constructor;
+  intro φ hφ F hF;
+  replace hF := Set.mem_setOf_eq.mp hF;
+  rcases (by simpa [buildAxioms] using hφ) with (rfl | rfl | rfl | rfl) <;> simp;
+
+instance : Entailment.Consistent InterpretabilityLogic.ILMinus_J5 := Veltman.consistent_of_sound_frameclass FrameClass.ILMinus_J5 $ by
+  use Veltman.trivialFrame;
+  apply Set.mem_setOf_eq.mpr;
+  infer_instance;
+
+end ILMinus_J5
+
+instance : InterpretabilityLogic.ILMinus ⪱ InterpretabilityLogic.ILMinus_J5 := by
+  constructor;
+  . apply weakerThan_of_subset_axioms $ by grind;
+  . apply Entailment.not_weakerThan_iff.mpr;
+    use (Axioms.J5 (.atom 0));
+    constructor;
+    . simp;
+    . apply Sound.not_provable_of_countermodel (𝓜 := Veltman.FrameClass.ILMinus);
+      apply Veltman.not_validOnFrameClass_of_exists_frame;
+      use {
+        toKripkeFrame := {
+          World := Fin 3
+          Rel := λ x y => x < y
+        }
+        isGL := Modal.Kripke.Frame.isGL_of_isFiniteGL {
+          trans := by omega;
+          irrefl := by omega;
+        }
+        S _ _ _ := False
+        S_cond := by tauto
+      }
+      constructor;
+      . tauto;
+      . by_contra hC;
+        replace hC := Veltman.Frame.HasAxiomJ5.of_validate_axiomJ5 hC |>.S_J5 (show 0 < 1 by omega) (show 1 < 2 by omega);
+        contradiction
+
+end LO.InterpretabilityLogic
